More theory of projections of the Aig

Valaig/Aig/Projections.lean
@@ -4,70 +4,125 @@ import all Valaig.Aig.Basic
 public import Valaig.Aig.Semantics
 public import Valaig.Aig.Iter
 
-public section
 namespace Valaig.Aig
 variable {aig : Aig} {wf : aig.WellFormed}
+
+namespace projectComb
+
+/--
+Construct a new Aig with the right amount of inputs added that will be required by `projectComb`.
+-/
+@[always_inline]
+def initLeaves (aig : Aig) (reset : Bool) : Aig :=
+  size.repeat (·.addInput.fst) .empty
+where
+  size := if reset then aig.numInputs else aig.numInputs + aig.numLatches
+
+variable {reset : Bool}
+
+attribute [local simp, local grind] initLeaves.size
+
+@[local simp, local grind .]
+theorem Comb_initLeaves :
+    (initLeaves aig reset).Comb := by
+  unfold initLeaves
+  induction initLeaves.size aig reset <;> grind [Nat.repeat]
+
+@[local simp, local grind .]
+theorem WellFormed_initLeaves :
+    (initLeaves aig reset).WellFormed := by
+  unfold initLeaves
+  induction initLeaves.size aig reset <;> grind [Nat.repeat]
+
+@[local simp, local grind =]
+theorem numInputs_initLeaves :
+  (initLeaves aig reset).numInputs = initLeaves.size aig reset := by
+  unfold initLeaves
+  induction initLeaves.size aig reset <;> grind [Nat.repeat]
+
+/--
+Maps an index from the original Aig to the one constructed by `initLeaves`.
+-/
+@[always_inline]
+def mapIdx (aig : Aig) (idx : LeafIdx) : InputIdx :=
+  match idx with
+  | .input idx => idx
+  | .latch idx => .ofIdx (idx.idx + aig.numInputs)
+
+theorem mapIdx_validIn_initLeaves_input {idx : InputIdx} (valid : idx.validIn aig) :
+    (mapIdx aig idx).validIn <| initLeaves aig reset := by
+  grind [InputIdx.validIn_eq, mapIdx]
+
+theorem mapIdx_validIn_initLeaves_latch {idx : LatchIdx} (valid : idx.validIn aig) :
+    (mapIdx aig idx).validIn <| initLeaves aig false := by
+  grind [InputIdx.validIn_eq, LatchIdx.validIn_eq, mapIdx]
+
+end projectComb
+
+attribute [local grind .] projectComb.WellFormed_initLeaves
+attribute [local grind .] projectComb.mapIdx_validIn_initLeaves_input
+attribute [local grind .] projectComb.mapIdx_validIn_initLeaves_latch
 
 /--
 Project out the reset and transition relation components of an Aig as new combinational Aigs.
 These may go in the future, replaced by better methods for going straight to SAT
 -/
-private def projectComb (aig : Aig) (reset : Bool) (wf : aig.WellFormed) : Aig × (Lit.In aig -> Lit) :=
-  go aig.iter .empty (.emptyWithCapacity aig.size)
+def projectComb (aig : Aig) (reset : Bool) (wf : aig.WellFormed) : Aig × (Lit.In aig -> Lit) :=
+  go aig.iter (projectComb.initLeaves aig reset) (.emptyWithCapacity aig.size)
 where
-  go iter (state : Aig) (map : Array Lit)
-    (size : iter.val.idx = map.size := by grind)
-    (valid : ∀ {lit} (_ : lit ∈ map), lit.validIn state := by grind) :=
-    match iter.step with
+  go it state (map : Array Lit)
+      (wf : state.WellFormed := by grind)
+      (inputMapsValid : {idx : InputIdx} → idx.validIn aig → (projectComb.mapIdx aig idx).validIn state := by grind)
+      (latchMapsValid : reset = false → {idx : LatchIdx} → idx.validIn aig → (projectComb.mapIdx aig idx).validIn state := by grind)
+      (valid : ∀ {lit} (_ : lit ∈ map), lit.validIn state := by grind)
+      (size : it.val.idx = map.size := by grind) :=
+    match it.step with
     | .done _ =>
-      ⟨state, fun lit => lit.val.mapTo <| map[lit.val.var.idx]'(by grind [Var.validIn_eq_lt_size])⟩
+      ⟨state, fun lit => lit.val.mapTo <| map[lit.val.var.idx]'(by grind [Var.validIn_eq])⟩
     | .yield it' var _ =>
-      let mapLit (lit : Lit) (h : lit.var < var := by grind) : Lit :=
-        lit.mapTo map[lit.var.idx]
+      let mapLit (lit : Lit) (h : lit.var < var := by grind) : Lit.In state :=
+        lit.mapTo map[lit.var.idx] |>.castIn state
 
       let res : Aig × Lit := 
         match _ : reset, _ : aig[var] with
-        | _, .false => (state, .false)
-        | _, .input _ | false, .latch _ =>
-          let (eq:=_) (state, idx) := state.addInput
-          (state, idx.getLit state)
-        | true, .latch idx => (state, mapLit <| idx.getReset aig)
-        | _, .and rhs0 rhs1 => state.addAnd (mapLit rhs0) (mapLit rhs1)
+        | _, .false =>         (state, .false)
+        | _, .input idx
+        | false, .latch idx => (state, (projectComb.mapIdx aig idx).getLit state)
+        | true, .latch idx =>  (state, mapLit <| idx.getReset aig)
+        | _, .and rhs0 rhs1 =>  state.addAnd (mapLit rhs0) (mapLit rhs1)
 
-      go it' res.fst (map.push res.snd) (by simp; grind) (by simp [res]; grind)
-  termination_by iter.finitelyManySteps
+      go it' res.fst (map.push res.snd)
+        (by subst res; grind only [usr WellFormed_addInput, usr WellFormed_addAnd])
+        (by subst res; grind only [= input_validIn_addInput_iff, = input_validIn_addAnd_iff])
+        (by subst res; grind only [= input_validIn_addInput_iff, = input_validIn_addAnd_iff])
+        (by subst res; grind)
+        (by subst res; grind only [Iter.val_yield, = Array.size_push])
+  termination_by it.finitelyManySteps
 
 section projectComb
-variable {reset : Bool} {state : Aig} {map : Array Lit} {iter : Std.Iter Var}
-variable {size : iter.val.idx = map.size}
+variable {reset : Bool} {wf : aig.WellFormed} {it : Std.Iter Var} {state : Aig} {map : Array Lit}
+variable {swf : state.WellFormed}
+variable {size : it.val.idx = map.size}
 
 @[local simp, local grind .]
-private theorem projectComb.Comb_go (comb : state.Comb) :
-    (go aig reset wf iter state map size valid).fst.Comb := by
+theorem projectComb.Comb_go (comb : state.Comb) :
+    (go aig reset wf it state map swf inputMapsValid latchMapsValid valid size).fst.Comb := by
   fun_induction go
-  · grind only
-  next res ih =>
-    apply ih
-    subst res
-    grind
+  next => assumption
+  next res ih => apply ih; subst res; grind
 
 @[local simp, local grind .]
-private theorem projectComb.WellFormed_go (swf : state.WellFormed) :
-    (go aig reset wf iter state map size valid).fst.WellFormed := by
-  fun_induction go
-  · grind only
-  next res ih =>
-    apply ih
-    subst res
-    grind
+theorem projectComb.WellFormed_go :
+    (go aig reset wf it state map swf inputMapsValid latchMapsValid valid size).fst.WellFormed := by
+  fun_induction go <;> assumption
 
 private theorem Comb_projectComb {reset} :
     (aig.projectComb reset wf).fst.Comb :=
-  projectComb.Comb_go (by simp)
+  projectComb.Comb_go projectComb.Comb_initLeaves
 
 private theorem WellFormed_projectComb {reset} :
     (aig.projectComb reset wf).fst.WellFormed :=
-  projectComb.WellFormed_go (by simp)
+  projectComb.WellFormed_go
 
 end projectComb
 
@@ -98,3 +153,9 @@ theorem Comb_transAig :
 theorem WellFormed_transAig :
     (aig.transAig wf).fst.WellFormed :=
   WellFormed_projectComb
+
+/--
+Map a leaf index from the original aig into the corresponding input to the result of `transAig`.
+-/
+def transAig.mapIdx (aig : Aig) (idx : LeafIdx) : InputIdx :=
+  projectComb.mapIdx aig idx
