Valaig/Aig/GetSet.lean
@@ -48,7 +48,7 @@ theorem get_eq_false_iff_isConstant {var : Var} (valid : var.validIn aig) :
     aig.get var = .false ↔ var = .constant := by
   have := aig.hconst
   simp_all [getElem_decls_eq_get, Var.constant_iff_idx_zero]
-  grind [Var, Var.validIn_of_lt_decls_size]
+  grind [Var, Var.lt_decls_size_of_validIn]
 
 /-
 Aig.empty Lemmas. There aren't many as the only valid ref/index is the constant
@@ -176,7 +176,7 @@ section aig
 -- These are needed for grind to reason about index validity
 attribute [local simp, local grind] Var.validIn InputIdx.validIn LatchIdx.validIn
 attribute [local simp, local grind] Aig.numInputs Aig.numLatches
-attribute [local grind →] Var.validIn_of_lt_decls_size
+attribute [local grind →] Var.lt_decls_size_of_validIn
 
 /-
 Aig.addInput Lemmas.
